ZFind_wbot.v
@@ -1,7 +1,7 @@
-Require Import ZF ZFpairs ZFsum ZFnats ZFrelations ZFord ZFfix ZFstable.
+Require Import ZF ZFpairs ZFnats ZFrelations ZFord ZFfix ZFstable.
 Require Import ZFgrothendieck.
-Require Import ZFlist ZFcoc.
-Import ZFrepl.
+Require Import ZFcoc.
+Require Import ZFwdom.
 Require Export ZFind_w.
 
 (** In this file we develop an alternative model of W-types where all stages are non-empty
@@ -17,130 +17,18 @@ Hypothesis Bm : morph1 B.
 
 Local Notation WF := (W_F A B).
 Local Notation Wd := (Wdom A B).
+Local Notation Wfb := (Wfbot A B).
 
-(** The type operator on the construction domain
-    (extended with bottom value) *)
+Hint Resolve Wintro_ext : core.
 
-  Lemma Wdom_cc_bot X :
-    X ⊆ Wd -> cc_bot X ⊆ Wd.
-red; intros.
-apply cc_bot_ax in H0; destruct H0; auto.
-rewrite H0; apply power_intro; intros.
-apply empty_ax in H1; contradiction.
+  Definition Wbot_ord := Ffix_ord Wfb Wd.
+
+  Lemma Wbot_o_o : isOrd Wbot_ord.
+apply Ffix_o_o; auto.
 Qed.
-
-  Definition W_F' X := W_F A B (cc_bot X).
-
-  Instance W_F'_mono : Proper (incl_set==>incl_set) W_F'.
-do 2 red; intros.
-unfold W_F'; apply W_F_mono; trivial.
-apply cc_bot_mono; auto with *.
-Qed.
-
-Lemma Wsup_ext' : forall X, ext_fun (W_F' X) (Wsup B).
-intros; unfold W_F'; apply Wsup_ext; trivial.
-Qed.
-Hint Resolve Wsup_ext' : core.
-
-Definition Wf' X := Wf A B (cc_bot X).
-
-Instance Wf_mono' : Proper (incl_set ==> incl_set) Wf'.
-do 2 red; intros.
-unfold Wf'; apply Wf_mono; trivial.
-apply cc_bot_mono; trivial.
-Qed.
-
-Instance Wf_morph' : morph1 Wf'.
-apply Fmono_morph; auto with *.
-Qed.
-Hint Resolve Wf_mono' Wf_morph' : core.
-
-Lemma Wsup_inj' : forall X Y x x',
-  X ⊆ Wd ->
-  Y ⊆ Wd ->
-  x ∈ W_F' X ->
-  x' ∈ W_F' Y ->
-  Wsup B x == Wsup B x' -> x == x'.
-intros X Y x x' tyf tyf' H H0 H1.
-apply Wsup_inj with (4:=H) (5:=H0) (6:=H1); trivial.
- apply Wdom_cc_bot; trivial.
- apply Wdom_cc_bot; trivial.
-Qed.
-
-Lemma Wsup_typ_gen' : forall X x,
-  X ⊆ Wd ->
-  x ∈ W_F' X ->
-  Wsup B x ∈ Wd.
-intros.
-apply Wsup_typ_gen with (3:=H0); trivial.
-apply Wdom_cc_bot; trivial.
-Qed.
-
-Lemma Wf_typ' : forall X,
-  X ⊆ Wd -> Wf' X ⊆ Wd.
-intros.
-unfold Wf'; apply Wf_typ; trivial.
-apply Wdom_cc_bot; trivial.
-Qed.
-Hint Resolve Wf_typ' : core.
-
-Lemma W_F_Wf_iso'' X :
-  X ⊆ Wd ->
-  iso_fun (W_F' X) (Wf' X) (Wsup B).
-split; intros.
- apply Wsup_morph; trivial.
-
- red; intros.
- apply Wf_intro; trivial.
-
- apply Wsup_inj' with X X; auto.
-
- unfold Wf' in H0; apply Wf_elim in H0; trivial.
- destruct H0; eauto with *.
-Qed.
-
-Lemma TI_Wf_typ' o :
-  isOrd o ->
-  TI Wf' o ⊆ Wd.
-induction 1 using isOrd_ind; intros.
-red; intros.
-apply TI_elim in H2; auto.
-destruct H2.
-revert H3; apply Wf_typ'; auto.
-Qed.
-
-
-  Lemma mt_not_in_W_F' o x :
-    isOrd o ->
-    x ∈ TI W_F' o ->
-    ~ x == empty.
-red; intros.
-apply TI_elim in H0; auto with *.
-destruct H0 as (o',?,?).
-unfold W_F' in H2.
-apply W_F_elim in H2; trivial.
-destruct H2 as (_,(_,?)).
-rewrite H2 in H1.
-symmetry in H1; apply discr_mt_couple in H1; trivial.
-Qed.
-
-  Lemma mt_not_in_Wf' o x :
-    isOrd o ->
-    x ∈ TI Wf' o ->
-    ~ x == empty.
-red; intros.
-apply TI_elim in H0; auto with *.
-destruct H0 as (o',?,?).
-unfold Wf' in H2; apply Wf_elim in H2; trivial.
-destruct H2 as (w,_,?).
-rewrite H2 in H1; apply empty_ax with (couple Nil (fst w)).
-rewrite <- H1.
-apply union2_intro1.
-apply singl_intro.
-Qed.
-
+  
 Lemma cc_bot_stable :
-  stable_class (fun X => X ⊆ Ffix Wf' Wd) cc_bot.
+  stable_class (fun X => X ⊆ Ffix Wfb Wd) cc_bot.
 unfold cc_bot; apply union2_stable_disjoint.
  do 2 red; reflexivity.
 
@@ -155,24 +43,11 @@ unfold cc_bot; apply union2_stable_disjoint.
  rewrite H1 in H2; apply H0 in H2.
  rewrite Ffix_def in H2; auto.
  destruct H2.
- apply mt_not_in_Wf' in H3; auto with *.
+ apply mt_not_in_Wfbot in H3; auto with *.
 Qed.
 
-Lemma W_F_stable' : stable_class (fun X => X ⊆ Ffix Wf' Wd) W_F'.
-apply compose_stable_class with (F:=WF) (K1:=fun _ => True); trivial.
- do 2 red; reflexivity.
-
- apply W_F_mono; trivial.
-
- apply cc_bot_morph.
-
- apply W_F_stable; trivial.
-
- apply cc_bot_stable.
-Qed.
-
-Lemma Wf_stable' : stable_class (fun X => X ⊆ Ffix Wf' Wd) Wf'.
-apply compose_stable_class with (F:=Wf A B) (K1:=fun X => X ⊆ cc_bot (Ffix Wf' Wd)); trivial.
+Lemma Wfbot_stable : stable_class (fun X => X ⊆ Ffix Wfb Wd) Wfb.
+apply compose_stable_class with (F:=Wf A B) (K1:=fun X => X ⊆ cc_bot (Ffix Wfb Wd)); trivial.
  do 2 red; intros.
  rewrite H; reflexivity.
 
@@ -190,31 +65,104 @@ apply compose_stable_class with (F:=Wf A B) (K1:=fun X => X ⊆ cc_bot (Ffix Wf'
  intros; apply cc_bot_mono; trivial.
 Qed.
 
-  Definition W_ord' := Ffix_ord Wf' Wd.
+  
+  Definition W_Fbot X := W_F A B (cc_bot X).
+  Definition Wibot o := TI W_Fbot o.
+  Definition Wbot := Wibot Wbot_ord  .
+  
+  Instance W_Fbot_mono : Proper (incl_set==>incl_set) W_Fbot.
+do 2 red; intros.
+unfold W_Fbot; apply W_F_mono; trivial.
+apply cc_bot_mono; auto with *.
+Qed.
 
-Lemma W_F_Wf_iso''' o f :
-  isOrd o ->
-  iso_fun (TI W_F' o) (TI Wf' o) f ->
-  iso_fun (W_F' (TI W_F' o)) (Wf' (TI Wf' o)) (wiso B (fbot f)).
+Lemma W_Fbot_stable : stable_class (fun X => X ⊆ Ffix Wfb Wd) W_Fbot.
+apply compose_stable_class with (F:=WF) (K1:=fun _ => True); trivial.
+ do 2 red; reflexivity.
+
+ apply W_F_mono; trivial.
+
+ apply cc_bot_morph.
+
+ apply W_F_stable; trivial.
+
+ apply cc_bot_stable.
+Qed.
+
+  Lemma mt_not_in_W_Fbot o x :
+    isOrd o ->
+    x ∈ Wibot o ->
+    ~ x == empty.
+red; intros.
+apply TI_elim in H0; auto with *.
+destruct H0 as (o',?,?).
+unfold W_Fbot in H2.
+apply W_F_elim in H2; trivial.
+destruct H2 as (_,(_,?)).
+rewrite H2 in H1.
+symmetry in H1; apply discr_mt_couple in H1; trivial.
+Qed.
+
+Lemma Wintro_inj_bot : forall X Y x x',
+  X ⊆ Wd ->
+  Y ⊆ Wd ->
+  x ∈ W_Fbot X ->
+  x' ∈ W_Fbot Y ->
+  Wintro x == Wintro x' -> x == x'.
+intros X Y x x' tyf tyf' H H0 H1.
+apply Wintro_inj with (4:=H) (5:=H0) (6:=H1); trivial.
+ apply Wdom_cc_bot; trivial.
+ apply Wdom_cc_bot; trivial.
+Qed.
+
+
+Lemma Wintro_typ_gen_bot : forall X x,
+  X ⊆ Wd ->
+  x ∈ W_Fbot X ->
+  Wintro x ∈ Wd.
 intros.
-apply iso_fun_trans with (W_F' (TI Wf' o)).
- unfold W_F' at 1 3; apply WFmap_iso; trivial.
- apply iso_cc_bot; trivial.
-  intro h; apply mt_not_in_W_F' in h; auto with *.
-  intro h; apply mt_not_in_Wf' in h; auto with *.
+apply Wf_intro in H0;[|trivial].
+revert H0; apply Wfbot_typ; trivial.
+Qed.
 
- apply W_F_Wf_iso''.
- apply TI_Wf_typ'; trivial.
+Lemma W_F_Wf_iso_bot X :
+  X ⊆ Wd ->
+  iso_fun (W_Fbot X) (Wfb X) Wintro.
+split; intros.
+ apply Wintro_morph.
+
+ red; intros.
+ apply Wf_intro; trivial.
+
+ apply Wintro_inj_bot with X X; auto.
+
+ apply Wf_elim in H0; trivial.
+ destruct H0; eauto with *.
+Qed.
+
+Lemma W_F_Wf_iso_bot' o f :
+  isOrd o ->
+  iso_fun (Wibot o) (TI Wfb o) f ->
+  iso_fun (W_Fbot (Wibot o)) (Wfb (TI Wfb o)) (wiso B (fbot f)).
+intros.
+apply iso_fun_trans with (W_Fbot (TI Wfb o)).
+ apply WFmap_iso; trivial.
+ apply iso_cc_bot; trivial.
+  intro h; apply mt_not_in_W_Fbot in h; auto with *.
+  intro h; apply mt_not_in_Wfbot in h; auto with *.
+
+ apply W_F_Wf_iso_bot.
+ apply TI_Wfbot_typ; trivial.
 Qed.
 
 Lemma wisobot_ext : forall X f f',
   ~ empty ∈ X ->
-  eq_fun X f f' -> eq_fun (W_F' X) (wiso B (fbot f)) (wiso B (fbot f')).
+  eq_fun X f f' -> eq_fun (W_Fbot X) (wiso B (fbot f)) (wiso B (fbot f')).
 red; intros.
 unfold wiso,comp_iso.
 assert (eqbot : eq_fun (cc_bot X) (fbot f) (fbot f')).
  apply eqf_fbot; trivial.
-apply Wsup_morph; trivial.
+apply Wintro_morph; trivial.
 apply WFmap_ext with (A:=A); intros; trivial.
  apply W_F_elim with (2:=H1); trivial.
 
@@ -234,47 +182,45 @@ apply cond_set_morph; auto.
 rewrite H1; reflexivity.
 Qed.
 
-Lemma TI_W_F_Wf_iso' o :
+Lemma TI_W_F_Wf_iso_bot o :
   isOrd o ->
-  iso_fun (TI W_F' o) (TI Wf' o) (TI_iso W_F' (fun f => wiso B (fbot f)) o).
+  iso_fun (Wibot o) (TI Wfb o) (TI_iso W_Fbot (fun f => wiso B (fbot f)) o).
 intros.
 apply TI_iso_fun; intros; auto.
- unfold W_F'; do 2 red; intros; apply W_F_mono; trivial.
+ unfold W_Fbot; do 2 red; intros; apply W_F_mono; trivial.
  apply cc_bot_mono; trivial.
 
  apply wisobot_ext; trivial.
- intros h; apply mt_not_in_W_F' in h; auto with *.
+ intros h; apply mt_not_in_W_Fbot in h; auto with *.
 
- apply W_F_Wf_iso'''; trivial.
+ apply W_F_Wf_iso_bot'; trivial.
 Qed.
 
-  Lemma W_fix' :
-    TI W_F' W_ord' == W_F' (TI W_F' W_ord').
-rewrite TI_iso_fixpoint with (2:=Wf_mono') (g:=fun f => wiso B (fbot f)); trivial.
+  Lemma Wbot_fix :
+    Wibot Wbot_ord == W_Fbot (Wibot Wbot_ord).
+unfold Wibot.
+rewrite TI_iso_fixpoint with (2:=Wfbot_mono A _ Bm) (g:=fun f => wiso B (fbot f)); trivial.
  apply TI_clos_fix_eqn; auto.
- apply Wf_stable'.
+ apply Wfbot_stable.
 
- apply W_F'_mono.
+ apply W_Fbot_mono.
 
  intros.
  apply wisobot_ext; trivial.
- intros h; apply mt_not_in_W_F' in h; auto with *.
+ intros h; apply mt_not_in_W_Fbot in h; auto with *.
 
- apply W_F_Wf_iso'''.
+ apply W_F_Wf_iso_bot'.
 
- apply Ffix_o_o; trivial.
- apply Wf_typ'.
+ apply Ffix_o_o; auto with *.
 Qed.
 
-  Lemma W_stages' o :
-    isOrd o ->
-    TI W_F' o ⊆ TI W_F' W_ord'.
+  Lemma Wbot_stages o : isOrd o -> Wibot o ⊆ Wbot.
 induction 1 using isOrd_ind; intros.
 red; intros.
 apply TI_elim in H2; auto with *.
 destruct H2 as (o',?,?).
-rewrite W_fix'.
-revert H3; apply W_F'_mono; auto.
+rewrite Wbot_fix.
+revert H3; apply W_Fbot_mono; auto.
 Qed.
 
 
@@ -290,21 +236,37 @@ Section W_Univ.
   Hypothesis aU : A ∈ U.
   Hypothesis bU : forall a, a ∈ A -> B a ∈ U.
 
-  Lemma G_W_F' X : X ∈ U -> W_F' X ∈ U.
+  Lemma G_W_Fbot X : X ∈ U -> W_Fbot X ∈ U.
 intros.
-unfold W_F'.
+unfold W_Fbot.
 apply G_W_F; trivial.
 apply G_union2; trivial.
 apply G_singl; trivial.
 apply G_incl with X; trivial.
 Qed.
 
-  Lemma G_W_ord' : W_ord' ∈ U.
-unfold W_ord'.
+  Lemma G_Wbot_ord : Wbot_ord ∈ U.
 apply G_Ffix_ord; auto.
 apply G_Wdom; trivial.
 Qed.
 
+  Lemma G_Wbot : Wbot ∈ U.
+apply G_TI; auto with *.
+ apply Wbot_o_o.
+
+ apply G_Wbot_ord.
+
+ apply G_W_Fbot.
+Qed.
+
+  Lemma G_Wibot o : isOrd o -> Wibot o ∈ U.
+intros.
+apply G_incl with Wbot; trivial.
+ apply G_Wbot.    
+
+ apply Wbot_stages; trivial.
+Qed.
+  
 End W_Univ.
 
 End W_theory.
